Final preparations for Shanghai Summer School.

theories/theories/utp_boyle.thy
@@ -14,48 +14,81 @@ abbreviation "p \<equiv> MkRealV ''p'' True"
 
 abbreviation "V \<equiv> MkRealV ''V'' True"
 
+text {* Signature *}
+
+definition Init :: "real \<Rightarrow> real \<Rightarrow> 'a WF_PREDICATE" where
+"Init ki Vi = `($k = \<guillemotleft>ki\<guillemotright>) \<and> ($k\<acute> = \<guillemotleft>ki\<guillemotright>) 
+            \<and> ($V = \<guillemotleft>Vi\<guillemotright>) \<and> ($V\<acute> = \<guillemotleft>Vi\<guillemotright>)
+            \<and> ($p = \<guillemotleft>ki / Vi\<guillemotright> \<and> $p\<acute> = \<guillemotleft>ki / Vi\<guillemotright>)`"
+
+definition ChangePressure :: "real \<Rightarrow> 'a WF_PREDICATE" where
+"ChangePressure dp = `p := $p + \<guillemotleft>dp\<guillemotright> ; V := (($k * $V) / ($k + ($V * \<guillemotleft>dp\<guillemotright>)))`"
+
+definition ChangeVolume :: "real \<Rightarrow> 'a WF_PREDICATE" where
+"ChangeVolume dV = `V := $V + \<guillemotleft>dV\<guillemotright> ; p := (($k * $p) / ($k + ($p * \<guillemotleft>dV\<guillemotright>)))`"
+
+declare Init_def [eval,evalr]
+declare ChangePressure_def [eval,evalr]
+declare ChangeVolume_def [eval,evalr]
+
 text {* Healthiness condition *}
 
-definition "BH(\<phi>) = `(\<exists> k. \<phi>) \<and> ($k = $p * $V)`"
+definition "BH1(\<phi>) = `(\<exists> k. \<phi>) \<and> ($k = $p * $V)`"
 
-declare BH_def [eval]
+definition "BH2(\<phi>) = `(\<exists> k\<acute>. \<phi>) \<and> ($k\<acute> = $p\<acute> * $V\<acute>)`"
 
-lemma BH_idem: "BH(BH(\<phi>)) = BH(\<phi>)"
+definition "BH3(\<phi>) = `\<phi> \<and> $k\<acute> = $k`"
+
+declare BH1_def [eval,evalr]
+declare BH2_def [eval,evalr]
+declare BH3_def [eval,evalr]
+
+lemma BH1_idem: "BH1(BH1(\<phi>)) = BH1(\<phi>)"
 proof -
-  have "BH(BH(\<phi>)) = `(\<exists> k. BH(\<phi>)) \<and> ($k = $p * $V)`"
-    by (simp add:BH_def)
+  have "BH1(BH1(\<phi>)) = `(\<exists> k. BH1(\<phi>)) \<and> ($k = $p * $V)`"
+    by (simp add:BH1_def)
 
   also have "... = `(\<exists> k. ((\<exists> k. \<phi>) \<and> ($k = $p * $V))) \<and> ($k = $p * $V)`"
-    by (simp add:BH_def)
+    by (simp add:BH1_def)
 
   also have "... = `(\<exists> k. \<phi>) \<and> ($k = $p * $V)`"
     by (utp_pred_auto_tac)
 
-  also have "... = BH(\<phi>)"
-    by (simp add:BH_def)
+  also have "... = BH1(\<phi>)"
+    by (simp add:BH1_def)
 
   finally show ?thesis ..
 qed
 
-lemma BH_idem_alt: "BH(BH(\<phi>)) = BH(\<phi>)"
+lemma BH1_idem_alt: "BH1(BH1(\<phi>)) = BH1(\<phi>)"
+  by (utp_pred_auto_tac)
+
+lemma BH2_idem: "BH2(BH2(\<phi>)) = BH2(\<phi>)"
+  by (utp_pred_auto_tac)
+
+lemma BH3_idem: "BH3(BH3(\<phi>)) = BH3(\<phi>)"
   by (utp_pred_auto_tac)
 
 lift_definition BOYLE :: "'a WF_THEORY" 
-is "({vs. {k\<down>, p\<down>, V\<down>} \<subseteq> vs}, {BH})"
+is "({vs. {k\<down>, p\<down>, V\<down>} \<subseteq> vs}, {BH1,BH2,BH3})"
   apply (auto simp add:WF_THEORY_def IDEMPOTENT_OVER_def)
-  apply (simp add:BH_idem)
+  apply (simp_all add:BH1_idem BH2_idem BH3_idem)
 done
 
 abbreviation "WF_BOYLE \<equiv> THEORY_PRED BOYLE"
 
-text {* Observations *}
-
-lemma BH_example_1:
-  "`($p = \<guillemotleft>10\<guillemotright>) \<and> ($V = \<guillemotleft>5\<guillemotright>) \<and> ($k = \<guillemotleft>50\<guillemotright>)` is BH"
+lemma Init_BH1:
+  "Vi > 0 \<Longrightarrow> (Init ki Vi) is BH1"
   by (utp_pred_auto_tac)
 
-lemma BH_example_2:
-  "`($p = \<guillemotleft>7\<guillemotright>) \<and> ($V = \<guillemotleft>3\<guillemotright>) \<and> ($k = \<guillemotleft>21\<guillemotright>)` is BH"
+text {* Observations *}
+
+lemma BH1_example_1:
+  "`($p = \<guillemotleft>10\<guillemotright>) \<and> ($V = \<guillemotleft>5\<guillemotright>) \<and> ($k = \<guillemotleft>50\<guillemotright>)` is BH1"
+  by (utp_pred_auto_tac)
+
+lemma BH1_example_2:
+  "`($p = \<guillemotleft>7\<guillemotright>) \<and> ($V = \<guillemotleft>3\<guillemotright>) \<and> ($k = \<guillemotleft>21\<guillemotright>)` is BH1"
   by (utp_pred_auto_tac)
 
 end
